bedrock2/src/bedrock2/ToCString.v
@@ -1,71 +1,105 @@
 Require Import bedrock2.Syntax bedrock2.Variables. Import bopname.
 Require Import coqutil.Datatypes.ListSet.
-Require Import Coq.ZArith.BinIntDef Coq.Numbers.BinNums Coq.Numbers.DecimalString.
-Require Import Coq.Strings.String. Local Open Scope string_scope.
+Require Import Coq.ZArith.BinIntDef Coq.Numbers.BinNums Coq.Numbers.DecimalString Strings.HexString.
+Require Import Coq.Strings.String. Import Byte. Local Open Scope string_scope.
 
-Definition prelude := "#include <stdint.h>
+Definition prelude := "// Generated from Bedrock code. Avoid editing directly.
+#include <stdint.h>
 #include <string.h>
 #include <assert.h>
 
-static __attribute__((constructor)) void _br2_preconditions(void) {
-  static_assert(~(intptr_t)0 == -(intptr_t)1, ""two's complement"");
-  assert(((void)""two's complement"", ~(intptr_t)0 == -(intptr_t)1));
-  uintptr_t u = 1;
-  assert(((void)""little-endian"", 1 == *(unsigned char *)&u));
-  intptr_t i = 1;
-  assert(((void)""little-endian"", 1 == *(unsigned char *)&i));
+#define BR_WORD_MAX UINTPTR_MAX
+typedef uintptr_t br_word_t;
+typedef intptr_t br_signed_t;
+
+static_assert(sizeof(br_word_t) == sizeof(br_signed_t), ""signed size"");
+static_assert(UINTPTR_MAX <= BR_WORD_MAX, ""pointer fits in int"");
+static_assert(~(br_signed_t)0 == -(br_signed_t)1, ""two's complement"");
+
+#if __STDC_VERSION__ >= 202311L && __has_include(<stdbit.h>)
+  #include <stdbit.h>
+  static_assert(__STDC_ENDIAN_NATIVE__ == __STDC_ENDIAN_LITTLE__, ""little-endian"");
+#elif defined(__GNUC__) && defined(__BYTE_ORDER__) && defined(__ORDER_LITTLE_ENDIAN__)
+  static_assert(__BYTE_ORDER__ == __ORDER_LITTLE_ENDIAN__, ""little-endian"");
+#elif defined(_MSC_VER) && !defined(__clang__) &&                              \
+    (defined(_M_IX86) || defined(_M_X64) || defined(_M_ARM) || defined(_M_ARM64))
+  // these MSVC targets are little-endian
+#else
+  #error ""failed to confirm that target is little-endian""
+#endif
+
+// ""An object shall have its stored value accessed only ... a character type.""
+static inline br_word_t _br_load1(br_word_t a) {
+  return *((uint8_t *)a);
 }
 
-// We use memcpy to work around -fstrict-aliasing.
-// A plain memcpy is enough on clang 10, but not on gcc 10, which fails
-// to infer the bounds on an integer loaded by memcpy.
-// Adding a range mask after memcpy in turn makes slower code in clang.
-// Loading individual bytes, shifting them together, and or-ing is fast
-// on clang and sometimes on GCC, but other times GCC inlines individual
-// byte operations without reconstructing wider accesses.
-// The little-endian idiom below seems fast in gcc 9+ and clang 10.
-static inline  __attribute__((always_inline, unused))
-uintptr_t _br2_load(uintptr_t a, uintptr_t sz) {
-  switch (sz) {
-  case 1: { uint8_t  r = 0; memcpy(&r, (void*)a, 1); return r; }
-  case 2: { uint16_t r = 0; memcpy(&r, (void*)a, 2); return r; }
-  case 4: { uint32_t r = 0; memcpy(&r, (void*)a, 4); return r; }
-  case 8: { uint64_t r = 0; memcpy(&r, (void*)a, 8); return r; }
-  default: __builtin_unreachable();
-  }
+static inline br_word_t _br_load2(br_word_t a) {
+  uint16_t r = 0;
+  memcpy(&r, (void *)a, sizeof(r));
+  return r;
 }
 
-static inline __attribute__((always_inline, unused))
-void _br2_store(uintptr_t a, uintptr_t v, uintptr_t sz) {
-  memcpy((void*)a, &v, sz);
+static inline br_word_t _br_load4(br_word_t a) {
+  uint32_t r = 0;
+  memcpy(&r, (void *)a, sizeof(r));
+  return r;
 }
 
-static inline __attribute__((always_inline, unused))
-uintptr_t _br2_mulhuu(uintptr_t a, uintptr_t b) {
-  #if (UINTPTR_MAX == (UINTMAX_C(1)<<31) - 1 + (UINTMAX_C(1)<<31))
+static inline br_word_t _br_load(br_word_t a) {
+  br_word_t r = 0;
+  memcpy(&r, (void *)a, sizeof(r));
+  return r;
+}
+
+static inline void _br_store1(br_word_t a, uint8_t v) {
+  *((uint8_t *)a) = v;
+}
+
+static inline void _br_store2(br_word_t a, uint16_t v) {
+  memcpy((void *)a, &v, sizeof(v));
+}
+
+static inline void _br_store4(br_word_t a, uint32_t v) {
+  memcpy((void *)a, &v, sizeof(v));
+}
+
+static inline void _br_store(br_word_t a, br_word_t v) {
+  memcpy((void *)a, &v, sizeof(v));
+}
+
+static inline br_word_t _br_mulhuu(br_word_t a, br_word_t b) {
+  #if BR_WORD_MAX == UINT32_MAX
 	  return ((uint64_t)a * b) >> 32;
-  #elif (UINTPTR_MAX == (UINTMAX_C(1)<<63) - 1 + (UINTMAX_C(1)<<63))
+  #elif BR_WORD_MAX == UINT64_MAX && (defined(__GNUC__) || defined(__clang__))
     return ((unsigned __int128)a * b) >> 64;
+  #elif defined(_M_X64)
+    uint64_t hi;
+    _umul128(a, b, &hi);
+    return hi;
+  #elif defined(_M_ARM64)
+    return __umulh(a, b);
   #else
-    #error ""32-bit or 64-bit uintptr_t required""
+    // See full_mul.v
+    br_word_t hh, lh, hl, low, second_halfword_w_oflow, n, ll, M;
+    n = ((((0u-(br_word_t)0x1)>>27)&0x3f)+0x1)>>1;
+    M = ((br_word_t)0x1<<n)-0x1;
+    ll = (a&M)*(b&M);
+    lh = (a&M)*(b>>n);
+    hl = (a>>n)*(b&M);
+    hh = (a>>n)*(b>>n);
+    second_halfword_w_oflow = ((ll>>n)+(lh&M))+(hl&M);
+    return ((hh+(lh>>n))+(hl>>n))+(second_halfword_w_oflow>>n);
   #endif
 }
 
-static inline __attribute__((always_inline, unused))
-uintptr_t _br2_divu(uintptr_t a, uintptr_t b) {
+static inline br_word_t _br_divu(br_word_t a, br_word_t b) {
   if (!b) return -1;
   return a/b;
 }
 
-static inline __attribute__((always_inline, unused))
-uintptr_t _br2_remu(uintptr_t a, uintptr_t b) {
+static inline br_word_t _br_remu(br_word_t a, br_word_t b) {
   if (!b) return a;
   return a%b;
-}
-
-static inline __attribute__((always_inline, unused))
-uintptr_t _br2_shamt(uintptr_t a) {
-  return a&(sizeof(uintptr_t)*8-1);
 }
 ".
 
@@ -74,13 +108,20 @@ Definition LF : string := String (Coq.Strings.Ascii.Ascii false true false true 
 Definition c_var := @id string.
 Definition c_fun := @id string.
 
-Definition c_lit w := "(uintptr_t)(UINTMAX_C(" ++ DecimalString.NilZero.string_of_int (BinInt.Z.to_int w) ++ "))".
-Definition c_byte_withoutcast b := DecimalString.NilZero.string_of_uint (BinNatDef.N.to_uint (Byte.to_N b)).
+Definition c_lit w := 
+  let s := if Z.ltb (Z.abs w) 0xff
+    then DecimalString.NilZero.string_of_int (BinInt.Z.to_int w)
+    else HexString.of_Z w in
+    let endswith_e s := Byte.eqb (List.last (list_byte_of_string s) "_"%byte) "e"%byte in
+    let s := if endswith_e s then s++" " else s in (* 0xe+1 --> invalid suffix on integer constant *)
+  if Z.ltb w 0
+  then "#error ""C does not support negative literals (" ++ s ++ ")"""
+  else s.
 
 Definition c_op1 op e :=
   match op with
   | op1.not => "~"++e
-  | op1.opp => "-"++e
+  | op1.opp => "0u-" ++ e (* silence MSVC warning C4146 *)
   end%string.
 
 Definition c_bop e1 op e2 :=
@@ -88,39 +129,69 @@ Definition c_bop e1 op e2 :=
   | add => e1++"+"++e2
   | sub => e1++"-"++e2
   | mul => e1++"*"++e2
-  | mulhuu => "_br2_mulhuu(" ++ e1 ++ ", " ++ e2 ++ ")"
-  | divu => "_br2_divu(" ++ e1 ++ ", " ++ e2 ++ ")"
-  | remu => "_br2_remu(" ++ e1 ++ ", " ++ e2 ++ ")"
+  | mulhuu => "_br_mulhuu(" ++ e1 ++ ", " ++ e2 ++ ")"
+  | divu => "_br_divu(" ++ e1 ++ ", " ++ e2 ++ ")"
+  | remu => "_br_remu(" ++ e1 ++ ", " ++ e2 ++ ")"
   | and => e1++"&"++e2
   | or => e1++"|"++e2
   | xor => e1++"^"++e2
-  | sru => e1++">>"++"_br2_shamt"++e2
-  | slu => e1++"<<"++"_br2_shamt"++e2
-  | srs => "(uintptr_t)((intptr_t)"++e1++">>"++"_br2_shamt"++e2++")"
-  | lts => "(uintptr_t)((intptr_t)"++e1++"<"++"(intptr_t)"++e2++")"
-  | ltu => "(uintptr_t)("++e1++"<"++e2++")"
-  | eq => "(uintptr_t)("++e1++"=="++e2++")"
+  | sru => e1++">>"++e2
+  | slu => e1++"<<"++e2
+  | srs => "(br_word_t)((br_signed_t)"++e1++">>"++e2++")"
+  | lts => "(br_word_t)((br_signed_t)"++e1++"<"++"(br_signed_t)"++e2++")"
+  | ltu => "(br_word_t)("++e1++"<"++e2++")"
+  | eq => "(br_word_t)("++e1++"=="++e2++")"
   end%string.
 
-Definition c_size (s : access_size) : string :=
+(* for load1, load2, load4, load, etc *)
+Definition size_suffix (s : access_size) : string :=
   match s with
   | access_size.one => "1"
   | access_size.two => "2"
   | access_size.four => "4"
-  | access_size.word => "sizeof(uintptr_t)"
+  | access_size.word => ""
   end.
 
+Definition c_inlinetable t :=
+  "static const uint8_t _inlinetable["++c_lit (Z.of_nat (List.length t))++"] = {"++
+      concat ", " (List.map HexString.of_N (List.map Byte.to_N t))++"};".
+Definition c_loadtable s i :=
+  "_br_load"++size_suffix s++"((br_word_t)&_inlinetable["++i++"])".
+
 Fixpoint c_expr (e : expr) : string :=
+  let p_expr e := match e with (* parenthesized expression *)
+                  | expr.literal _ | expr.var _ => c_expr e
+                  | expr.op1 _ _ (* MSVC *) | _ => "(" ++ c_expr e ++ ")"
+                  end in
+  let p_operand2 e := match e with (* e is passed to binary operator whose 1st*)
+    (* operand is a br_word_t, so if it is a literal, we can avoid a cast per *)
+    (* usual arithmetic conversions. E.g. [a+5] instead of [a+(br_word_t)5]. *)
+                      | expr.literal v => c_lit v
+                      | _ => p_expr e
+                  end in
+  let p_shamt e := match e with (* shift amount, safely truncated *)
+                   | expr.literal v =>
+                   if (Z.leb 0 v && Z.ltb v 32)%bool then c_lit v
+                   else    "("++p_expr e++"&(sizeof(br_word_t)*8-1))"
+                   | _ =>  "("++p_expr e++"&(sizeof(br_word_t)*8-1))"
+                   end in
   match e with
-  | expr.literal v => c_lit v
+  | expr.literal v => "(br_word_t)" ++ c_lit v
   | expr.var x => c_var x
-  | expr.load s ea => "_br2_load(" ++ c_expr ea ++ ", " ++ c_size s++ ")"
-  | expr.inlinetable s t index => "({ static const uint8_t _inlinetable["++c_lit (Z.of_nat (List.length t))++"] = {"++concat ", " (List.map c_byte_withoutcast t)++"}; _br2_load((uintptr_t)&_inlinetable["++c_expr index++"], "++c_size s++"); })"
-  | expr.op1 op e1 => c_op1 op ("(" ++ c_expr e1 ++ ")")
-  | expr.op op e1 e2 => c_bop ("(" ++ c_expr e1 ++ ")") op ("(" ++ c_expr e2 ++ ")")
-  | expr.lazy_and e1 e2 => "(" ++ c_expr e1 ++ ") && (" ++ c_expr e2 ++ ")"
-  | expr.lazy_or e1 e2 => "(" ++ c_expr e1 ++ ") || (" ++ c_expr e2 ++ ")"
-  | expr.ite c e1 e2 => "(" ++ c_expr c ++ ") ? (" ++ c_expr e1 ++ ") : (" ++ c_expr e2 ++ ")"
+  | expr.load s ea => "_br_load" ++ size_suffix s++ "(" ++ c_expr ea ++ ")"
+  | expr.inlinetable s t index =>  (* x = tbl[i] is handled in [c_cmd]. GNUC fallback: *)
+    "({ " ++ c_inlinetable t ++ c_loadtable s (c_expr index) ++ "; })"
+  | expr.op1 op e1 => c_op1 op (p_expr e1)
+  | expr.op op e1 e2 =>
+    match op with
+    | slu | sru | srs => c_bop (p_expr e1) op (p_shamt e2)
+    | add | sub | mul
+    | and | or  | xor => c_bop (p_expr e1) op (p_operand2 e2)
+    | _  => c_bop (p_expr e1) op (p_expr e2)
+    end
+  | expr.lazy_and e1 e2 => p_expr e1 ++ " && " ++ p_expr e2
+  | expr.lazy_or e1 e2 => p_expr e1 ++ " || " ++ p_expr e2
+  | expr.ite c e1 e2 => p_expr c ++ " ? " ++ p_expr e1 ++ " : " ++ p_expr e2
   end.
 
 Fixpoint List_uniq {A} (eqb : A -> A -> bool) (l : list A) :=
@@ -147,12 +218,16 @@ Definition c_act := c_call.
 Fixpoint c_cmd (indent : string) (c : cmd) : string :=
   match c with
   | cmd.store s ea ev
-    => indent ++ "_br2_store(" ++ c_expr ea ++ ", " ++ c_expr ev ++ ", " ++ c_size s ++ ");" ++ LF
+    => indent ++ "_br_store" ++ size_suffix s ++ "(" ++ c_expr ea ++ ", " ++ c_expr ev ++ ");" ++ LF
   | cmd.stackalloc x n body =>
-    let tmp := "_br2_stackalloc_"++x in (* might shadow if not fresh, likely type error... *)
-    indent ++ "{ uint8_t "++tmp++"["++c_lit n++"] = {0}; "++x++" = (uintptr_t)&"++tmp++";"++LF++
-    c_cmd indent body ++
-    indent ++ "}" ++ LF
+    (* Extend the lifetime of the allocation until the end of ambient block,
+     * favoring readability over timely deallocation (which clang et al don't
+     * do anyway. However, name collisions can cause compilation errors. *)
+    let tmp := "_br_stackalloc_"++x in
+    indent ++ "uint8_t "++tmp++"["++c_lit n++"] = {0}; "++x++" = (br_word_t)&"++tmp++";"++LF++
+    c_cmd indent body
+  | cmd.set x (expr.inlinetable s t ei) =>
+  indent ++ "{ " ++ c_inlinetable t ++ " " ++ x ++ " = " ++ c_loadtable s (c_expr ei) ++ "; }" ++ LF
   | cmd.set x ev =>
     indent ++ c_var x ++ " = " ++ c_expr ev ++ ";" ++ LF
   | cmd.unset x =>
@@ -199,8 +274,8 @@ Definition fmt_c_decl (rett : string) (args : list String.string) (name : String
     (match args, retptrs with
     | nil, nil => "void"
     | _, _ => concat ", " (
-        List.map (fun a => "uintptr_t "++c_var a) args ++
-        List.map (fun r => "uintptr_t* "++c_var r) retptrs)
+        List.map (fun a => "br_word_t "++c_var a) args ++
+        List.map (fun r => "br_word_t* "++c_var r) retptrs)
     end)
   in
   (rett ++ " " ++ c_fun name ++ "(" ++ argstring ++ ")").
@@ -211,7 +286,7 @@ Definition c_decl (f : String.string * func) :=
   | nil => fmt_c_decl "void" args name nil
   | cons _ _ =>
     let retrenames := fst (rename_outs (List.removelast rets) (cmd.vars body)) in
-     fmt_c_decl "uintptr_t" args name (List.map snd retrenames)
+     fmt_c_decl "br_word_t" args name (List.map snd retrenames)
   end ++ ";".
 
 
@@ -223,7 +298,7 @@ Definition c_func '(name, (args, rets, body)) :=
     let r0 := List.last rets r0 in
     let rets' := List.removelast rets in
     let retrenames := fst (rename_outs rets' (cmd.vars body)) in
-    (fmt_c_decl "uintptr_t" args name (List.map snd retrenames), Some r0, retrenames)
+    (fmt_c_decl "br_word_t" args name (List.map snd retrenames), Some r0, retrenames)
   end in
   let decl := fst (fst decl_retvar_retrenames) in
   let retvar := snd (fst decl_retvar_retrenames) in
@@ -233,7 +308,7 @@ Definition c_func '(name, (args, rets, body)) :=
       (List_minus String.eqb allvars args)) in
   decl ++ " {" ++ LF ++
     let indent := "  " in
-    (match localvars with nil => "" | _ => indent ++ "uintptr_t " ++ concat ", " (List.map c_var localvars) ++ ";" ++ LF end) ++
+    (match localvars with nil => "" | _ => indent ++ "br_word_t " ++ concat ", " (List.map c_var localvars) ++ ";" ++ LF end) ++
     c_cmd indent body ++
     concat "" (List.map (fun '(o, optr) => indent ++ "*" ++ c_var optr ++ " = " ++ c_var o ++ ";" ++ LF) retrenames) ++
     indent ++ "return" ++ (match retvar with None => "" | Some rv => " "++c_var rv end) ++ ";" ++ LF ++
