bedrock2/src/bedrock2/ToCStringTest.v
@@ -1,0 +1,27 @@
+Require Import bedrock2.Syntax bedrock2.NotationsCustomEntry.
+
+Import Syntax.Coercions BinInt String List.ListNotations.
+Local Open Scope string_scope. Local Open Scope Z_scope. Local Open Scope list_scope.
+
+Definition main := func! () ~> (r) {
+  r = $0;
+  v = $(expr.inlinetable access_size.one [Byte.x00; Byte.x01] 1);
+  require v;
+
+  require $(expr.inlinetable access_size.one [Byte.x00; Byte.x01] 1);
+
+  stackalloc 1 as p;
+  store1(p, $1);
+  require load1(p);
+
+  require (p+$1 == $1 + p);
+  require (p*$1 == $1 * p);
+  require (p<<$31 == (p&$1) * $(2^31));
+
+  r = $1
+}.
+
+From coqutil.Macros Require Import WithBaseName.
+From bedrock2 Require Import ToCString.
+
+Definition test := String.list_byte_of_string (c_module &[,main]).
